app/Decode.v
@@ -1,0 +1,58 @@
+From ExtLib Require Export
+     Applicative.
+From JSON Require Export
+     Decode.
+From App Require Export
+     AppMessage.
+Export
+  ApplicativeNotation.
+
+Instance JDecode__Request : JDecode (swap_request id) :=
+  fun j =>
+    m <- dpath "method" j;;
+    match m with
+    | "clean"       => ret Request__Clean
+    | "listAccount" => Request__ListAccount <$> dpath "user" j
+    | "takeOrder"   => liftA2 Request__TakeOrder (dpath "user" j) (dpath "order" j)
+    | "makeOrder"   => liftA2 Request__MakeOrder (dpath "user" j)
+                             (dpath "buyTicker" j) <*> (dpath "buyAmount" j) <*>
+                             (dpath "sellTicker" j) <*> (dpath "sellAmount" j)
+    | "deposit"     => liftA2 Request__Deposit (dpath "user" j) (dpath "ticker" j)
+                             <*> (dpath "amount" j)
+    | "withdraw"    => liftA2 Request__Withdraw (dpath "user" j) (dpath "ticker" j)
+                             <*> (dpath "amount" j)
+    | _             => ret Request__ListOrders
+    end.
+
+Instance JDecode__Account : JDecode (accountT id) :=
+  fun j =>
+    aid <- dpath "ID"          j;;
+    uid <- dpath "UserID"      j;;
+    tcr <- dpath "AssetTicker" j;;
+    amt <- dpath "Amount"      j;;
+    ret (aid, (uid, tcr, amt)).
+
+Instance JDecode__Order : JDecode (orderT id) :=
+  fun j =>
+    oid <- dpath "ID"         j;;
+    bid <- dpath "BuyerID"    j;;
+    bam <- dpath "BuyAmount"  j;;
+    sid <- dpath "BuyerID"    j;;
+    sam <- dpath "SellAmount" j;;
+    ret (oid, (bid, bam, sid, sam)).
+
+Instance JDecode__Response : JDecode (swap_response id) :=
+  fun j =>
+    c <- dpath "code" j;;
+    match c with
+    | 200 =>
+      Response__ListAccount <$> dpath' decode__list "accounts" j <|>
+      Response__ListOrders  <$> dpath' decode__list "orders"   j <|>
+      Response__Account     <$> decode j                       <|>
+      Response__Order       <$> decode j
+    | 204 => ret Response__NoContent
+    | 400 => ret Response__BadRequest
+    | 402 => ret Response__InsufficientFund
+    | 404 => ret Response__NotFound
+    | _   => ret Response__InternalServerError
+    end.
